semantics/il1/bigstep_il1Script.sml
@@ -1,0 +1,81 @@
+open HolKernel boolLib bossLib listTheory Parse IndDefLib finite_mapTheory relationTheory arithmeticTheory ast_l1Theory bigstep_l1Theory pred_setTheory pairTheory lcsymtacs integerTheory ast_il1Theory;
+
+val _ = new_theory "bigstep_il1";
+
+val (bs_il1_expr_rules, bs_il1_expr_ind, bs_il1_expr_cases) = Hol_reln `
+    (* Values *)
+    (!v s.bs_il1_expr (IL1_Value v, s) v) /\
+
+    (* Plus *)
+    (!e1 e2 n1 n2 s.
+        (bs_il1_expr (e1, s) (IL1_Integer n1) /\
+         bs_il1_expr (e2, s) (IL1_Integer n2))
+     ==> bs_il1_expr (IL1_Plus e1 e2, s) (IL1_Integer (n1 + n2))) /\
+
+    (* Geq *)
+    (!e1 e2 n1 n2 s.
+        (bs_il1_expr (e1, s) (IL1_Integer n1) /\
+         bs_il1_expr (e2, s) (IL1_Integer n2))
+     ==> bs_il1_expr (IL1_Geq e1 e2, s) (IL1_Boolean (n1 >= n2))) /\
+
+    (* Deref *)
+    (!l s.
+        l ∈ FDOM s
+    ==> bs_il1_expr (IL1_Deref l, s) (IL1_Integer (s ' l))) /\
+
+    (* EIf *)
+    (!e1 e2 e3 s v.
+        (bs_il1_expr (e1, s) (IL1_Boolean T) /\
+         bs_il1_expr (e2, s) v)
+     ==> bs_il1_expr (IL1_EIf e1 e2 e3, s) v) /\
+
+    (!e1 e2 e3 s v.
+        (bs_il1_expr (e1, s) (IL1_Boolean F) /\
+         bs_il1_expr (e3, s) v)
+     ==> bs_il1_expr (IL1_EIf e1 e2 e3, s) v)`;
+
+val (bs_il1_rules, bs_il1_ind, bs_il1_cases) = Hol_reln `
+    (*  Expressions *)
+    (!e v s.
+        bs_il1_expr (e, s) v
+    ==> bs_il1 (IL1_Expr e, s) v s) /\
+
+    (* Assign *)
+    (!l e s n.
+       (User l ∈ FDOM s /\
+        bs_il1_expr (e, s) (IL1_Integer n))
+    ==> bs_il1 (IL1_Assign (User l) e, s) IL1_ESkip (s |+ (User l, n))) /\
+
+    (!l e s n.
+        bs_il1_expr (e, s) (IL1_Integer n)
+    ==> bs_il1 (IL1_Assign (Compiler l) e, s) IL1_ESkip (s |+ (Compiler l, n))) /\
+
+    (* Seq *)
+    (!e1 e2 v s s' s''.
+        (bs_il1 (e1, s) IL1_ESkip s' /\
+         bs_il1 (e2, s') v s'')
+     ==> bs_il1 (IL1_Seq e1 e2, s) v s'') /\
+
+    (* SIf *)
+    (!e1 e2 e3 v s s'.
+        (bs_il1_expr (e1, s) (IL1_Boolean T) /\
+         bs_il1 (e2, s) v s')
+     ==> bs_il1 (IL1_SIf e1 e2 e3, s) v s') /\
+
+    (!e1 e2 e3 v s s'.
+        (bs_il1_expr (e1, s) (IL1_Boolean F) /\
+         bs_il1 (e3, s) v s')
+     ==> bs_il1 (IL1_SIf e1 e2 e3, s) v s') /\
+
+    (* While *)
+    (!e1 e2 s s' s''.
+        (bs_il1_expr (e1, s) (IL1_Boolean T) /\
+         bs_il1 (e2, s) IL1_ESkip s' /\
+         bs_il1 (IL1_While e1 e2, s') IL1_ESkip s'')
+     ==> bs_il1 (IL1_While e1 e2, s) IL1_ESkip s'') /\
+
+    (!e1 e2 s.
+       (bs_il1_expr (e1, s) (IL1_Boolean F))
+    ==> bs_il1 (IL1_While e1 e2, s) IL1_ESkip s)`;
+
+val _ = export_theory ();
